disk-betree/BlockCache.dfy
@@ -7,10 +7,10 @@ abstract module BlockCache {
   type View<T> = imap<Reference, T>
     
   function ViewOf<T>(k: Constants, s: Variables) : View
-    
-  function Read<T>(k: Constants, s: Variables, ref: Reference) : T
-    requires ref in ViewOf(k, s)
-    ensures Read(k, s, ref) == ViewOf(k, s)[ref];
+  
+  // function Read<T>(k: Constants, s: Variables, ref: Reference) : T
+  //   requires ref in ViewOf(k, s)
+  //   ensures Read(k, s, ref) == ViewOf(k, s)[ref];
     
   datatype CacheOp<T> =
     | AllocOp(block: T, successors: iset<Reference>, new_ref: Reference)
@@ -24,20 +24,16 @@ abstract module BlockCache {
   }
     
   predicate Apply(k: Constants, s: Variables, s': Variables, op: CacheOp)
-    requires op.AllocOp? ==> op.new_ref !in ViewOf(k, s)
     ensures Apply(k, s, s', op) ==> ViewOf(k, s') == ApplyToView(ViewOf(k, s), op)
+    ensures op.AllocOp? && Apply(k, s, s', op) ==> op.new_ref !in ViewOf(k, s)
+    ensures op.WriteOp? && Apply(k, s, s', op) ==> op.ref in ViewOf(k, s)
     
   predicate Apply2(k: Constants, s: Variables, s': Variables, op1: CacheOp, op2: CacheOp)
-    requires op1.AllocOp? ==> op1.new_ref !in ViewOf(k, s)
-    requires op2.AllocOp? ==> op2.new_ref !in ApplyToView(ViewOf(k, s), op1)
     ensures Apply2(k, s, s', op1, op2) ==> ViewOf(k, s') == ApplyToView(ApplyToView(ViewOf(k, s), op1), op2)
   {
-    exists sint :: 
+    exists sint ::
       && Apply(k, s, sint, op1)
-      && assert ViewOf(k, sint) == ApplyToView(ViewOf(k, s), op1);
       && Apply(k, sint, s', op2)
-      && assert ViewOf(k, s') == ApplyToView(ViewOf(k, sint), op2);
-      && true
   }
     
   function Root(k: Constants) : Reference
